theories/imports.v
@@ -2,13 +2,18 @@ From Coq Require Export ssreflect ssrbool.
 From Coq Require Export Logic.PropExtensionality
   (propositional_extensionality) Program.Basics (const) FunInd.
 From Equations Require Export Equations.
+Require Export Autosubst2.syntax Autosubst2.core Autosubst2.unscoped.
+Export CombineNotations.
+Derive NoConfusion for Ty.
+Derive NoConfusion for Ki.
+Derive NoConfusion for Tm.
+
+
 From Hammer Require Export Tactics.
 From stdpp Require Export relations (rtc, rtc_transitive, rtc_once, rtc_inv, rtc(..), diamond, confluent, diamond_confluent, sn) base(sum_relation(..)).
 Require Export Psatz.
 
 Global Set Warnings "-notation-overridden".
-Require Export Autosubst2.syntax Autosubst2.core Autosubst2.unscoped.
-Export CombineNotations.
 
 (* Notation "s [ sigmatm ]" := (subst_Term sigmatm s) (at level 7, left associativity) : subst_scope. *)
 (* Notation "s ⟨ xitm ⟩" := (ren_Term xitm s) (at level 7, left associativity) : subst_scope. *)
