theories/par.v
@@ -53,6 +53,10 @@ where "a ⇒ b" := (Par a b).
 
 Infix "⇒*" := (rtc Par) (at level 70, no associativity).
 
+Definition ICoherent A0 A1 : Prop :=
+  exists B, rtc TyPar A0 B /\ rtc TyPar A1 B.
+
+
 Lemma par_refl a : a ⇒ a.
 Proof. elim : a; eauto with par. Qed.
 
@@ -283,8 +287,6 @@ Qed.
 Lemma C_App : ltac2:(gen_cong P_App Coherent).
 Proof. hauto lq:on use:PS_App unfold:Coherent. Qed.
 
-Definition ICoherent A0 A1 : Prop :=
-  exists B, rtc TyPar A0 B /\ rtc TyPar A1 B.
 
 (* Lemma pars_pi_inv A B U : *)
 (*   Pi A B ⇒* U -> exists A0 B0, U = Pi A0 B0 /\ A ⇒* A0 /\ B ⇒* B0. *)
